\documentclass[11pt]{article}
\usepackage{amssymb}
\usepackage{amsthm}
\usepackage{enumitem}
\usepackage{amsmath}
\usepackage{bm}
\usepackage{adjustbox}
\usepackage{mathrsfs}
\usepackage{graphicx}
\usepackage{siunitx}
\usepackage{physics}
\usepackage[mathscr]{euscript}

\title{\textbf{Solved selected problems of Lagrangian and Hamiltonian by Mann}}
\author{Franco Zacco}
\date{}

\addtolength{\topmargin}{-3cm}
\addtolength{\textheight}{3cm}

\newcommand{\N}{\mathbb{N}}
\newcommand{\Z}{\mathbb{Z}}
\newcommand{\R}{\mathbb{R}}
\newcommand{\C}{\mathbb{C}}
\newcommand{\hatr}{\bm{\hat{r}}}
\newcommand{\hatx}{\bm{\hat{x}}}
\newcommand{\haty}{\bm{\hat{y}}}
\newcommand{\hatz}{\bm{\hat{z}}}
\newcommand{\hatth}{\bm{\hat{\theta}}}
\newcommand{\hatphi}{\bm{\hat{\phi}}}
\newcommand{\hatrho}{\bm{\hat{\rho}}}
\newcommand{\ei}[1]{\vec{\bm{e}}_#1}
\theoremstyle{definition}
\newtheorem*{solution*}{Solution}
\renewcommand*{\proofname}{\textbf{Solution}}

\begin{document}
\maketitle
\thispagestyle{empty}

\begin{proof}{\textbf{5.2}}
From equation (5.0.26) we have that
\begin{align*}
    \sum_{j=0}^\infty (j+2)(j+1)a_{j+2}x^j
    - \sum_{j=0}^\infty j(j-1)a_{j}x^j
    - 2\sum_{j=0}^\infty ja_{j}x^j
    + \lambda(\lambda + 1)\sum_{j=0}^\infty a_{j}x^j
    = 0
\end{align*}
Then
\begin{align*}
    \sum_{j=0}^\infty \bigg[(j+2)(j+1)a_{j+2}
    - j(j-1)a_{j}
    - 2ja_{j}
    + \lambda(\lambda + 1)a_{j}
    \bigg]x^j
    = 0
\end{align*}
So, must be that
\begin{align*}
    (j+2)(j+1)a_{j+2} - j(j-1)a_{j} - 2ja_{j} + \lambda(\lambda + 1)a_{j}
    &= 0\\
    (j+2)(j+1)a_{j+2} + a_j(-j(j-1) - 2j + \lambda(\lambda + 1))
    &= 0\\
    (j+2)(j+1)a_{j+2} + a_j(-j^2 - j - \lambda j + \lambda^2 + \lambda + \lambda j)
    &= 0\\
    (j+2)(j+1)a_{j+2} + a_j(-j(j + 1 + \lambda) + \lambda(\lambda + 1 + j))
    &= 0\\
    (j+2)(j+1)a_{j+2} + a_j(\lambda-j)(j + 1 + \lambda)
    &= 0
\end{align*}
Where we added and subtracted $\lambda j$ in the third step. Hence
\begin{align*}
    a_{j+2} &= - \frac{(\lambda-j)(\lambda + j + 1)}{(j+2)(j+1)}a_j
\end{align*}
Which is the expected recurrence formula.
\end{proof}

\end{document}